Add files via upload

Tarea3/T3/CWSS.dfy
@@ -14,9 +14,20 @@ method Main() {
 
     var base : real := baseFindig * attackSurface * environmental;
     print base;
+
+    print "\nTotal:";
+    assert zero <= baseFindig <= hundred;
+    assert zero <= attackSurface <= one;
+    assert zero <= environmental <= one;
+    var total := funcTotal(baseFindig, attackSurface, environmental);
+    print total;
 }
 
 const hundred : real := 100.0;
+const ninetyfive : real := 95.0;
+const eigthy : real := 80.0;
+const sixty : real := 60.0;
+const fourty : real := 40.0;
 const twenty : real := 20.0;
 const fifteen : real := 15.0;
 const ten : real := 10.0;
@@ -29,12 +40,13 @@ const twenty_multiplier : real := 0.05;
 const minimum : real := 0.01;
 
 method funcImpact(impact:real) returns (result:real)
-    requires zero <= impact && impact <= one
+    requires zero == impact || zero < impact <= one
+    requires one == impact || zero <= impact < one
     ensures impact == zero ==> result == zero
     ensures impact != zero ==> result == one
-    ensures result >= zero && result <= one
+    ensures zero == result || one == result
 {
-    assert zero <= impact && impact <= one;
+    assert zero == impact || zero < impact <= one;
     if impact == zero { result:= zero; } else { result:= one; }
     assert impact == zero ==> result == zero;
     assert impact != zero ==> result == one;
@@ -49,16 +61,16 @@ method funcBaseFinding(ti:real, ap:real, al:real, ic:real, fc:real) returns (bas
     ensures zero <= baseFinding <= hundred
 {
     var fti := funcImpact(ti);
-    assert zero <= fti <= one;
+    var formulaBase := ((ten*ti) + (five*(ap+al)) + (five*fc));
     
-    baseFinding := zero;
-    if (fti * ic > zero) {     
-        baseFinding := (((ten*ti) + (five*(ap+al)) + (five*fc)) * ic) * four;
-        
-        if baseFinding < zero { baseFinding:= zero; } 
-        else if baseFinding > hundred { baseFinding := hundred; }
-        else { baseFinding := baseFinding; }
-    }
+    assert zero <= fti <= one;
+    if (fti * ic == zero) { baseFinding := zero; }
+    else if (fti * ic == one) { baseFinding := formulaBase * four; }
+    else if ( fti == one && zero < ic <= one ) { baseFinding := (formulaBase * ic) * four; }
+
+    if baseFinding < zero { baseFinding:= zero; } 
+    else if baseFinding > hundred { baseFinding := hundred; }
+    else { baseFinding := baseFinding; }   
 }
 
 method funcAttackSurface(rp:real, rl:real, av:real, asn:real, lin:real, sc:real) returns (attackSurface:real) 
@@ -70,20 +82,28 @@ method funcAttackSurface(rp:real, rl:real, av:real, asn:real, lin:real, sc:real)
     requires zero <= sc <= one
     ensures zero <= attackSurface <= one
 {
-    var block1 := (rp + rl + av);
-    var block2 := (twenty * block1);
-    var block3 := (twenty * sc);
-    var block4 := (fifteen * lin);
-    var block5 := (five * asn);
-    var block6 := (block2 + block3);
-    var block7 := (block6 + block4);
-    var block8 := (block7 + block5);
-    attackSurface := (block8 / hundred);
-    assert zero <= attackSurface <= one ==> (attackSurface / hundred) <= one;   
+    var accumulator := (twenty*rp);
+    assert zero <= accumulator <= twenty;
+    accumulator := accumulator + (twenty*rl);
+    assert zero <= accumulator <= fourty;
+    accumulator := accumulator + (twenty*av);
+    assert zero <= accumulator <= sixty;
+    accumulator := accumulator + (twenty*sc);
+    assert zero <= accumulator <= eigthy;
+    accumulator := accumulator + (fifteen*lin);
+    assert zero <= accumulator <= ninetyfive;
+    accumulator := accumulator + (five*asn);  
+    assert zero <= accumulator <= hundred;  
+    attackSurface := accumulator * minimum; 
+    assert zero <= attackSurface <= one;  
+
+    if attackSurface < zero { attackSurface:= zero; assert accumulator == zero; }
+    else if attackSurface > one { attackSurface := one; assert accumulator == one; }
+    else { attackSurface := attackSurface; assert zero <= attackSurface <= one; }
 } 
 
 method funcEnvironmental(bi:real, di:real, ex:real, ec:real, p:real) returns (environmental:real) 
-    requires zero <= bi <= one
+    requires zero <= bi <= one 
     requires zero <= di <= one
     requires zero <= ex <= one
     requires zero <= ec <= one
@@ -91,31 +111,32 @@ method funcEnvironmental(bi:real, di:real, ex:real, ec:real, p:real) returns (en
     ensures zero <= environmental <= one
 {
     var fbi := funcImpact(bi);
-    var result := (ten*bi) + (three*di) + (four*ex) + (three*p);
+    assert bi == zero ==> bi == zero;
+    assert zero == fbi || one == fbi;
+    var formulaBase := (ten*bi) + (three*di) + (four*ex) + (three*p);
+    assert zero <= formulaBase <= twenty;
 
+    environmental := formulaBase;
+    if (zero < fbi < one) { environmental := environmental * fbi; }
+    if (zero < ec < one) { environmental := environmental * ec; }
     if (fbi * ec == zero) { environmental := zero; }
-    else if (fbi * ec == one) { environmental := result * twenty_multiplier; }
-    else if fbi == one { environmental := (result * ec) * twenty_multiplier; }
+    else { environmental := environmental * twenty_multiplier; }
     
-    if environmental < zero { environmental:= zero; } 
-    else if environmental > one { environmental := one; }
-    else { environmental := environmental; }    
+    if environmental < zero { environmental:= zero; assert environmental == zero; } 
+    else if environmental > one { environmental := one; assert environmental == one; }
+    else { environmental := environmental; assert zero <= environmental <= one; }    
 } 
 
 method funcTotal(finding:real, surface:real, env:real) returns (cwss:real)
-    requires one <= finding <= hundred;
-    requires one <= surface <= one;
-    requires one <= env <= one;
-    ensures one <= cwss <= hundred;
+    requires zero <= finding <= hundred;
+    requires zero <= surface <= one;
+    requires zero <= env <= one;
+    ensures zero <= cwss <= hundred;
 {
-    cwss := surface * hundred;
-    assert zero <= cwss <= hundred;
-    cwss := (cwss * finding) * minimum;
-    assert zero <= cwss <= hundred;
-    cwss := cwss * env;
-    assert zero <= cwss <= hundred;
-
-    print cwss;
+    cwss := finding * surface * env;
+    if cwss < zero { cwss:= zero; assert cwss == zero; } 
+    else if cwss > one { cwss := one; assert cwss == one; }
+    else { cwss := cwss; assert zero <= cwss <= one; }    
 }
 
 
